@prefix solidhotel: <https://github.com/gergelyth/solid-hotel/blob/master/solidhotel.ttl#> .
@prefix rdf: <http://www.w3.org/1999/02/22-rdf-syntax-ns#> .
@prefix rdfs: <http://www.w3.org/2000/01/rdf-schema#> .
@prefix owl: <http://www.w3.org/2002/07/owl#> .
@prefix dcterms: <http://purl.org/dc/terms/> .
@prefix vann: <http://purl.org/vocab/vann/> .
@prefix schema: <https://schema.org/> .
@prefix solid: <http://www.w3.org/ns/solid/terms#> .

solidhotel: rdf:type owl:Ontology ;
    dcterms:title "Solid Hotel project ontology" ;
    dcterms:description "The ontology adding RDF terms required for the Solid Hotel project." ;
    vann:preferredNamespacePrefix "solidhotel" ;
    vann:preferredNamespaceURI <https://github.com/gergelyth/solid-hotel/blob/master/solidhotel.ttl#> .

### Classes
solidhotel:ReservationLink
    a rdfs:Class ;
    rdfs:comment "A resource containing information which helps to pair Solid Pods to reservations."@en ;
    rdfs:label "ReservationLink"@en .

solidhotel:PrivacyToken
    a rdfs:Class ;
    rdfs:comment "A resource helping to identify what personal information fields are kept at the hotel."@en ;
    rdfs:label "PrivacyToken"@en .

solidhotel:PrivacyTokenDeletion
    a rdfs:Class ;
    rdfs:comment "A resource containing information about the deletion request of a privacy token."@en ;
    rdfs:label "PrivacyTokenDeletion"@en .

solidhotel:ReservationStateChange
    a rdfs:Class ;
    rdfs:comment "A resource containing information about a reservation state change."@en ;
    rdfs:label "ReservationStateChange"@en .

### Enumerates
solidhotel:ReservationActive a schema:ReservationStatusType ;
    rdfs:label "ReservationActive"@en;
    rdfs:comment "The status for a currently active reservation where the guest is checked-in."@en .

solidhotel:ReservationPast a schema:ReservationStatusType ;
    rdfs:label "ReservationPast"@en ;
    rdfs:comment "The status for a reservation in the past where the guest has already checked-out"@en .

solidhotel:NotificationType a rdfs:Class ;
    rdfs:label "NotificationType"@en ;
    rdfs:comment "Enumerated type values for a Notification."@en ;
    rdfs:subClassOf schema:StatusEnumeration .

solidhotel:BookingRequestNotification a solidhotel:NotificationType ;
    rdfs:label "BookingRequestNotification"@en ;
    rdfs:comment "The notification submitted to the hotel to create a reservation"@en .

solidhotel:ReservationStateChangeNotification a solidhotel:NotificationType ;
    rdfs:label "ReservationStateChangeNotification"@en ;
    rdfs:comment "The notification requesting a reservation status change at the counterparty"@en .

solidhotel:FailureReportNotification a solidhotel:NotificationType ;
    rdfs:label "FailureReportNotification"@en ;
    rdfs:comment "The notification reporting an error to the counterparty"@en .

solidhotel:ProfileModificationNotification a solidhotel:NotificationType ;
    rdfs:label "ProfileModificationNotification"@en ;
    rdfs:comment "The notification reporting a change in a local guest profile to the counterparty"@en .

solidhotel:InitialPairingRequestNotification a solidhotel:NotificationType ;
    rdfs:label "InitialPairingRequestNotification"@en ;
    rdfs:comment "The notification which starts the reservation pairing operation"@en .

solidhotel:PairingRequestWithInformationNotification a solidhotel:NotificationType ;
    rdfs:label "PairingRequestWithInformationNotification"@en ;
    rdfs:comment "The notification completing the reservation pairing operation carrying the required data"@en .

solidhotel:PrivacyTokenNotification a solidhotel:NotificationType ;
    rdfs:label "PrivacyTokenNotification"@en ;
    rdfs:comment "The notification informing the counterparty about a personal information held"@en .

solidhotel:PrivacyTokenDeletionNotification a solidhotel:NotificationType ;
    rdfs:label "PrivacyTokenDeletionNotification"@en ;
    rdfs:comment "The notification submitted to request the removal of a personal information field"@en .

### Properties
solidhotel:isProcessed
    a rdf:Property ;
    rdfs:comment "Defines if the subject has been processed already."@en ;
    rdfs:label "isProcessed"@en .

solidhotel:notificationType
    a rdf:Property ;
    rdfs:comment "Defines the type of the notification"@en ;
    rdfs:label "notificationType"@en ;
    schema:domainIncludes solid:Notification ;
    schema:rangeIncludes solidhotel:NotificationType .

solidhotel:idDocumentType
    a rdf:Property ;
    rdfs:comment "Defines the identification document type of the person."@en ;
    rdfs:label "idDocumentType"@en .

solidhotel:idDocumentNumber
    a rdf:Property ;
    rdfs:comment "Defines the identification document number of the person."@en ;
    rdfs:label "idDocumentNumber"@en .

solidhotel:targetDataset
    a rdf:Property ;
    rdfs:comment "Refers to the target Solid dataset."@en ;
    rdfs:label "targetDataset"@en .

solidhotel:forHotel
    a rdf:Property ;
    rdfs:comment "Refers to the target hotel of the dataset."@en ;
    rdfs:label "forHotel"@en .

solidhotel:forReservation
    a rdf:Property ;
    rdfs:comment "Refers to the target reservation in the Solid Pod."@en ;
    rdfs:label "forReservation"@en .

solidhotel:targetFields
    a rdf:Property ;
    rdfs:comment "The array of the personal information fields targeted by this resource."@en ;
    rdfs:label "targetFields"@en .